Eliminate an admit by proving several extra lemmas

src/arch/Types_i.fst
@@ -192,3 +192,43 @@ let le_quad32_to_bytes_to_quad32 (s:seq nat8 { length s == 16 }) :
   ) else (
     assert (s == s')
   )
+
+let le_seq_quad32_to_bytes_of_singleton (q:quad32) :
+  Lemma (le_quad32_to_bytes q == le_seq_quad32_to_bytes (create 1 q))
+  =
+  four_to_seq_LE_is_seq_four_to_seq_LE q;
+  ()
+
+open FStar.Mul
+let slice_commutes_seq_four_to_seq_LE (#a:Type) (s:seq (four a)) (n:nat{n <= length s}) (n':nat{ n <= n' /\ n' <= length s}) :
+  Lemma(slice (seq_four_to_seq_LE s) (n * 4) (n' * 4) ==
+        seq_four_to_seq_LE (slice s n n'))
+  =
+  assert (equal (slice (seq_four_to_seq_LE s) (n * 4) (n' * 4))
+                (seq_four_to_seq_LE (slice s n n')));
+  ()
+
+let slice_commutes_le_seq_quad32_to_bytes (s:seq quad32) (n:nat{n <= length s}) (n':nat{ n <= n' /\ n' <= length s}) :
+  Lemma(slice (le_seq_quad32_to_bytes s) (n * 16) (n' * 16) ==
+        le_seq_quad32_to_bytes (slice s n n'))
+  =
+  slice_commutes_seq_four_to_seq_LE s n n';
+  assert (slice (seq_four_to_seq_LE s) (n * 4) (n' * 4) == seq_four_to_seq_LE (slice s n n'));
+(*
+  le_seq_quad32_to_bytes (slice s n n') == seq_four_to_seq_LE (seq_map (nat_to_four 8) (seq_four_to_seq_LE (slice s n n')));
+                                        == seq_four_to_seq_LE (seq_map (nat_to_four 8) (slice (seq_four_to_seq_LE s) (n * 4) (n' * 4))
+  slice (le_seq_quad32_to_bytes s) (n * 16) (n' * 16) 
+  ==  slice (seq_four_to_seq_LE (seq_map (nat_to_four 8) (seq_four_to_seq_LE s))) (n * 16) (n' * 16)
+  ==  seq_four_to_seq_LE (slice (seq_map (nat_to_four 8) (seq_four_to_seq_LE s)) (n * 4) (n' * 4))
+*)
+  slice_seq_map_commute (nat_to_four 8) (seq_four_to_seq_LE s) (n*4) (n'*4);
+
+  let s_inner = (seq_map (nat_to_four 8) (seq_four_to_seq_LE s)) in
+  slice_commutes_seq_four_to_seq_LE s_inner (n * 4) (n' * 4);
+  ()
+
+let slice_commutes_le_seq_quad32_to_bytes0 (s:seq quad32) (n:nat{n <= length s}) :
+  Lemma(slice (le_seq_quad32_to_bytes s) 0 (n * 16) ==
+        le_seq_quad32_to_bytes (slice s 0 n))
+  =
+  slice_commutes_le_seq_quad32_to_bytes s 0 n
